sketch of SepProver.

src/SepExpr.v
@@ -23,20 +23,21 @@ Module SepExpr (B : SepLog).
     }.
     Variable sfuncs : list ssignature.
 
+    Variable consts : list (PropX (tvarD pcType) (tvarD stateType)).
+
     Inductive sexpr : variables types -> Type :=
+    | Emp : forall vars, sexpr vars
     | Inj : forall vars, expr funcs vars None -> sexpr vars
     | Star : forall vars, sexpr vars -> sexpr vars -> sexpr vars
     | Exists : forall vars t, sexpr (t :: vars) -> sexpr vars
     | Cptr : forall vars, expr funcs vars pcType -> sexpr (stateType :: vars) -> sexpr vars
     | Func : forall vars (f : fin sfuncs), 
       hlist (expr funcs vars) (SDomain (get sfuncs f)) -> sexpr vars
-      (** TODO: This const case doesn't work because there is no (reasonable) semi-decidable equality on propX **)
-    | Const : forall vars, 
-      PropX (tvarD pcType) (tvarD stateType) -> sexpr vars
-    (** PtsTo should be derived, that way we can handle different sizes easily, 
-     ** baking it in allows us to derive <> facts from points to 
+    | Const : forall vars, fin consts -> sexpr vars
+    (** If PtsTo is derived: we can handle different sizes easily, 
+     ** If PtsTo is built-in: we can derive <> facts easily (also precision)
      **)
-      .
+    .
     (** NOTE: If I want to be able to reflect arbitrary propX terms (ExistsX,ForallX), then I'm going to need
      ** another index on sexpr to express the (type -> PropX)
      **)
@@ -49,10 +50,13 @@ Module SepExpr (B : SepLog).
         | Exists _ t b => fun g m => PropX.Exists (fun x : tvarD t => @sexprD _ b (HCons x g) m)
         | Func _ f b => fun g =>
           applyD (exprD g) b _ (SDenotation (get sfuncs f))
-        | Const _ p => fun g _ => p
+        | Const _ p => fun _ _ => (*p*)
+          get consts p
         | Star _ l r => fun g m => 
           PropX.Exists (fun ml : L.smem => PropX.Exists (fun mr : L.smem => 
-            PropX.And (PropX.Inj (L.split m ml mr)) (And (sexprD l g ml) (sexprD l g mr))))
+            PropX.And (PropX.Inj (L.split m ml mr)) (And (sexprD l g ml) (sexprD r g mr))))
+        | Emp _ => fun _ m => 
+          PropX.Inj (L.semp m)
         | Cptr _ p t => fun g m =>
           PropX.Cptr (exprD g p) 
           (fun x : tvarD stateType => PropX.Exists (fun m => 
@@ -63,6 +67,11 @@ Module SepExpr (B : SepLog).
       Definition sexprEq vars (a : sexpr vars) : forall b, option (a = b).
         refine ((fix sexprEq vars (a : sexpr vars) {struct a} : forall b, option (a = b) :=
           match a in sexpr vars return forall b : sexpr vars, option (a = b) with
+            | Emp _ => fun b =>
+              match b with
+                | Emp _ => Some _ 
+                | _ => None
+              end
             | Inj v l => fun b =>
               match b in sexpr v' return forall l : expr funcs v' None, option (Inj l = b) with
                 | Inj _ r => fun l => match exprEq l r with
@@ -165,14 +174,18 @@ Module SepExpr (B : SepLog).
                   end
                 | _ => fun _ _ => None
               end (refl_equal _) (hlistEq (@exprEq _ _ _) args)
-            | Const _ _ => fun _ => None
+            | Const _ x => fun b => 
+              match b with
+                | Const _ y => if finEq x y then Some _ else None
+                | _ => None
+              end
               (** TODO: Problem with Const **)
           end) vars a);
         clear sexprEq; try abstract (subst; reflexivity).
       Defined.
     End Eq.
 
-    Definition Himp (cs : codeSpec (tvarD pcType) (tvarD stateType)) (gl gr : sexpr nil) 
+    Definition Himp (cs : codeSpec (tvarD pcType) (tvarD stateType)) (gl gr : sexpr nil)
 (*      : PropX (tvarD pcType) (tvarD stateType) := *)
       : Prop :=
       L.himp (fun m => valid cs nil (sexprD gl HNil m)) (fun m => valid cs nil (sexprD gr HNil m)).
@@ -186,12 +199,13 @@ Module SepExpr (B : SepLog).
     Variable stateType : tvar types.
     Variable stateMem : tvarD stateType -> L.mem.
     Variable sfuncs : list (ssignature pcType stateType).
+    Variable consts : list (PropX (tvarD pcType) (tvarD stateType)).
     
     (** TODO: it looks like I need this in terms of PropX? **)
     Definition SProverT : Type := forall
       (cs : codeSpec (tvarD pcType) (tvarD stateType))
       (hyps : list (@Qexpr types funcs)) (** Guards **)
-      (gl gr : @sexpr types funcs pcType stateType sfuncs nil), 
+      (gl gr : @sexpr types funcs pcType stateType sfuncs consts nil), 
       option (Himp stateMem cs gl gr).
 
   End SProver.
@@ -203,17 +217,194 @@ Module SepExpr (B : SepLog).
     Variable stateType : tvar types.
     Variable stateMem : tvarD stateType -> L.mem.
     Variable sfuncs : list (ssignature pcType stateType).
+    Variable consts : list (PropX (tvarD pcType) (tvarD stateType)).
 
-    Definition BabySep : @SProverT types fs pcType stateType stateMem sfuncs.
-    red.
-    refine (fun _ _ gl gr =>
+    Definition ReflSep : @SProverT types fs pcType stateType stateMem sfuncs consts.
+    red. refine (fun _ _ gl gr =>
       if sexprEq gl gr then 
         Some _ 
       else 
         None).
     subst. unfold Himp. unfold L.himp. intros. auto.
-  Defined.
+    Defined.
+
+    Parameter dmap : forall (K : Type) (V : K -> Type), Type.
+    Parameter map : Type -> Type -> Type.
+
+    Parameter dmap_empty : forall K V, @dmap K V.
+    Parameter dmap_fold : forall {A} {K} {V} (f : A -> forall k, V k -> A) (a : A) (m : @dmap K V), A.
+    Parameter dmap_insert : forall {K} {V} k, V k -> @dmap K V -> dmap V.
+    Parameter dmap_join : forall {K} {V}, @dmap K V -> dmap V -> dmap V.
+    Parameter map_empty : forall K V, map K V.
+    Parameter map_fold : forall {A} {K} {V} (f : A -> K -> V -> A) (a : A) (m : map K V), A.
+    Parameter map_insert : forall {K} {V}, K -> V -> @map K V -> map K V.
+    Parameter map_join : forall {K} {V}, map K V -> @map K V -> map K V.
+
+    Parameter dmap_fold_empty : forall A K V f (a : A), dmap_fold f a (@dmap_empty K V) = a.
+    Parameter map_fold_empty : forall A K V f (a : A), map_fold f a (@map_empty K V) = a.
+
+    Record SHeap vars : Type :=
+    { funcs  : @dmap (fin sfuncs) (fun f => hlist (expr fs vars) (SDomain (get sfuncs f)))
+    ; cptrs  : map (expr fs vars pcType) (sexpr fs sfuncs consts (stateType :: vars))
+    ; pures  : list (expr fs vars None)
+    ; cnsts  : list (fin consts)
+    ; other  : list (sexpr fs sfuncs consts vars)
+    }.
+
+    Definition denote vars (h : SHeap vars) :  sexpr fs sfuncs consts vars :=
+      let acc := Emp _ _ _ _ in
+      let acc := dmap_fold (fun a x y => Star a (Func _ x y)) acc (funcs h) in
+      let acc := map_fold (fun a x y => Star a (Cptr x y)) acc (cptrs h) in
+      let acc := fold_left (fun a x => Star a (Inj _ _ x)) (pures h) acc in
+      let acc := fold_left (fun a x => Star a (Const _ _ _ x)) (cnsts h) acc in
+      fold_left (fun a x => Star a x) (other h) acc.
+
+    Fixpoint hash vars (s : sexpr fs sfuncs consts vars) : SHeap vars :=
+      match s in @sexpr _ _ _ _ _ _ vs return SHeap vs with
+        | Inj _ p => 
+          {| funcs := dmap_empty _
+           ; cptrs := map_empty _ _
+           ; pures := p :: nil
+           ; cnsts := nil
+           ; other := nil
+           |}
+        | Star _ l r => 
+          let ll := hash l in
+          let rr := hash r in
+          {| funcs := dmap_join (funcs ll) (funcs rr)
+           ; cptrs := map_join (cptrs ll) (cptrs rr)
+           ; pures := pures ll ++ pures rr
+           ; cnsts := cnsts ll ++ cnsts rr
+           ; other := other ll ++ other rr 
+          |}
+        | Func _ f args => 
+          {| funcs := dmap_insert f args (dmap_empty _)
+           ; cptrs := map_empty _ _ 
+           ; pures := nil
+           ; cnsts := nil
+           ; other := nil
+          |}
+        | Cptr _ p s => 
+          {| funcs := dmap_empty _
+           ; cptrs := map_insert p s (map_empty _ _)
+           ; pures := nil
+           ; cnsts := nil
+           ; other := nil
+          |}
+        | Emp _ => 
+          {| funcs := dmap_empty _
+           ; cptrs := map_empty _ _
+           ; pures := nil
+           ; cnsts := nil
+           ; other := nil
+           |}
+        | Const _ c =>
+          {| funcs := dmap_empty _
+           ; cptrs := map_empty _ _ 
+           ; pures := nil
+           ; cnsts := c :: nil
+           ; other := nil
+          |}
+        | x => 
+          (** TODO : Other cases are problematic... **)
+          {| funcs := dmap_empty _ ; cptrs := map_empty _ _ ; pures := nil ; cnsts := nil ; other := x :: nil |}
+      end.
+
+(*
+    Fixpoint hash_cc T vars (s : sexpr fs sfuncs consts vars) 
+      :  @dmap (fin sfuncs) (fun f => hlist (expr fs vars) (SDomain (get sfuncs f))) 
+      -> map (expr fs vars pcType) (sexpr fs sfuncs consts (stateType :: vars))
+      -> list (expr fs vars None)
+      -> (   @dmap (fin sfuncs) (fun f => hlist (expr fs vars) (SDomain (get sfuncs f))) 
+          -> map (expr fs vars pcType) (sexpr fs sfuncs consts (stateType :: vars))
+          -> list (expr fs vars None)-> T) -> T :=
+      match s in @sexpr _ _ _ _ _ _ vs 
+        return @dmap (fin sfuncs) (fun f => hlist (expr fs vs) (SDomain (get sfuncs f))) 
+        -> map (expr fs vs pcType) (sexpr fs sfuncs consts (stateType :: vs))
+        -> list (expr fs vs None)
+        -> (   @dmap (fin sfuncs) (fun f => hlist (expr fs vs) (SDomain (get sfuncs f))) 
+          -> map (expr fs vs pcType) (sexpr fs sfuncs consts (stateType :: vs))
+          -> list (expr fs vs None)-> T) -> T 
+        with
+        | Inj _ p => fun fs cps ps cc =>
+          cc fs cps (p :: ps)
+        | Star _ l r => fun fs cps ps cc =>
+          hash_cc l fs cps ps (fun a b c => hash_cc r a b c cc)
+        | Func _ f args => fun fs cps ps cc =>
+          cc (dmap_insert f args fs) cps ps 
+        | Cptr _ p s => fun fs cps ps cc =>
+          cc fs (map_insert p s cps) ps
+        | _ => fun fs cps ps cc =>
+          (** TODO : Other cases are problematic... **)
+          cc fs cps ps
+      end.
+*)
+
+    Lemma denote_hash : forall (s :sexpr fs sfuncs consts nil) cs, 
+      Himp stateMem cs (denote (hash s)) s.
+    Proof.
+      (** This is too weak, need to generalize with respect to the continuation,
+       ** should probably switch to non-cps for the time being... 
+       **)
+      unfold Himp. intros.
+      generalize (@HNil (option (@fin type types)) (@tvarD types)).
+      revert s.
+      unfold tvar.
+      generalize dependent (@nil (option (@fin type types))).
+      induction s; simpl; unfold denote, L.himp; simpl;
+        repeat rewrite map_fold_empty in *; repeat rewrite dmap_fold_empty in *; intuition.
+        (* *)
+        admit.
+        (* *)
+        unfold L.himp in *. admit.
+        (* *)
+(*
+        eapply Exists_E in H. eassumption. simpl. intros.
+        eapply Exists_E. simpl. econstructor. simpl. left. reflexivity. simpl.
+        intros. eapply And_E2. eapply And_E2. econstructor. simpl. left. 
+        eapply And_E2. eapply And_E2. eapply Exists_E in H.  eassumption. simpl.
+        
+
+        intros.
+        eapply Exists_I. 
+        
+
+        (** Admit *) admit.
+        unfold denote in *. simpl in H.
+        repeat eapply PropX.Exists_I.
+        repeat eapply PropX.And_I.
+*)
+    Admitted.
+
+    (** Procedure:
+     ** - Hash the left hand side
+     ** - ?? Handle implications...
+     ** - ?? Generate <> constraints ??
+     ** - For each right hand side conjunct
+     **   - if it is in the SHeap
+     **       cancel
+     **     else 
+     **       ?? is this automatically problematic, this procedure probably won't prove it
+     ** - Discharge pure constraints with solver...
+     **)
+
+    Goal forall cs (a : fin consts), 
+      Himp stateMem cs (Const fs sfuncs nil a) (Const fs sfuncs nil a).
+      intros.
+      pose (ReflSep cs nil (Const _ _ nil a) (Const _ _ nil a)). simpl in *.
+      (** Note: everything has to be concrete in order for simplification to work! **)
+      unfold ReflSep in *. unfold sexprEq in *.
+      destruct (finEq a a). simpl in *. 
+      match goal with
+        | [ H := Some ?X |- _ ] => generalize X
+      end. auto.
+      congruence.
+    Defined.
+
   End BabySep.
+
+  
+
 
   Section QSexpr.
     (** Guarded separation logic expressions **)
